Rename Related to RTC.

dfs.v
@@ -1,22 +1,30 @@
 (* A depth-first search algorithm. *)
 
-Require Import Utf8 List.
+Require Import Utf8 Wf_nat List.
 From larith Require Import tactics notations utilities.
 Import ListNotations.
 
-Section Related_elements.
+Section Reflexive_transitive_closure.
 
 Variable X : Type.
 Variable R : X -> X -> Prop.
 
-Inductive Related : list X -> Prop :=
-  | related_nil : Related []
-  | related_one x : Related [x]
-  | related_cons x y l : Related (y :: l) -> R x y -> Related (x :: y :: l).
+Inductive RTC : list X -> Prop :=
+  | rtc_refl x : RTC [x]
+  | rtc_cons x y l : RTC (y :: l) -> R x y -> RTC (x :: y :: l).
 
-End Related_elements.
+Theorem RTC_trans l1 x1 x2 l2 :
+  RTC (l1 ++ [x1]) -> RTC (x2 :: l2) -> R x1 x2 ->
+  RTC (l1 ++ x1 :: x2 :: l2).
+Proof.
+induction l1; simpl; intros. apply rtc_cons; easy.
+destruct l1; simpl in *; inv H; repeat apply rtc_cons.
+4: apply IHl1. all: easy.
+Qed.
 
-Arguments Related {_}.
+End Reflexive_transitive_closure.
+
+Arguments RTC {_}.
 
 Section Stateful_search.
 
@@ -73,37 +81,46 @@ Fixpoint dfs depth visited v : list node + list node :=
     end
   end.
 
-Definition Path := Related (λ v w, In w (adj v)).
 Notation diff x y := (subtract dec x y).
-Notation Inl x := (∃l, x = inl l).
+Notation Inr x := (∃r, x = inr r).
+Notation Path := (RTC (λ v w, In w (adj v))).
 
-Definition DFS_path visited tr :=
-  Path tr /\ NoDup tr /\ Forall (λ v, ¬In v visited) tr.
+Definition DFS_solution_weak v tr :=
+  Path (v :: tr) /\ accept (last tr v) = true.
 Definition DFS_solution visited v tr :=
-  DFS_path visited (v :: tr) /\ accept (last tr v) = true.
+  DFS_solution_weak v tr /\ Forall (λ v, ¬In v visited) (v :: tr).
 
-Theorem dfs_sound depth visited v tr :
-  dfs depth visited v = inr tr ->
-  DFS_solution visited v tr.
+Theorem dfs_sound_weak depth visited v tr :
+  dfs depth visited v = inr tr -> DFS_solution_weak v tr.
 Proof.
 revert visited v tr; induction depth; simpl; intros. easy.
 destruct (in_dec dec v visited). easy.
-destruct (accept v) eqn:C.
-- inv H; repeat split. apply related_one.
-  apply NoDup_cons; [easy|apply NoDup_nil].
-  apply Forall_cons; easy. apply C.
-- destruct (search _) eqn:Hs. easy. destruct p as [v' tr']; inv H.
-  apply search_sound with (P:=DFS_solution (v :: visited)) in Hs.
-  (* search_sound is not strong enough to handle cascading states. *)
-Admitted.
+destruct (accept v) eqn:C. inv H; split; [apply rtc_refl|apply C].
+destruct (search _) eqn:Hs. easy. destruct p as [v' tr']; inv H.
+apply search_sound with (P:=DFS_solution_weak) in Hs as [H []].
+split. apply rtc_cons; easy. rewrite last_cons; apply H1.
+apply IHdepth.
+Qed.
 
 Variable graph : list node.
 Hypothesis graph_spec : ∀v, In v graph.
 
-Theorem dfs_complete visited v :
-  Inl (dfs (length (diff graph visited)) visited v) ->
-  ¬∃tr, DFS_solution visited v tr.
+Theorem dfs_complete visited v tr :
+  DFS_solution visited v tr ->
+  Inr (dfs (length (diff graph visited)) visited v).
 Proof.
+remember (length (diff graph visited)) as n eqn:len;
+revert len; revert visited v tr.
+apply lt_wf_rect with (n:=n); clear n; intros; destruct n.
+- (* Contradition; v ∈ graph \ visited. *)
+  destruct H0 as [_ H0]; inv H0.
+  exfalso; apply in_nil with (a:=v).
+  apply eq_sym, length_zero_iff_nil in len; rewrite <-len.
+  apply subtract_spec; easy.
+- (* The search through (adj v) must yield a solution. *)
+  destruct H0; inv H1; simpl.
+  destruct (in_dec _) as [F|_]; [easy|].
+  destruct (accept v) eqn:Hv; [now exists []|].
 Admitted.
 
 End Depth_first_search.
